### Exercises 4.1-1
***
Show that the solution of ![](http://latex.codecogs.com/gif.latex? T\(n\) = T\(\\lceil n/2 \\rceil\) + 1) is O(lg n).

### `Answer`
我们猜想 ![](http://latex.codecogs.com/gif.latex? T\(n\) \\le c\\lg\(n-2\) )

![](http://latex.codecogs.com/gif.latex? T\(n\) = T\(\\lceil n/2 \\rceil\) + 1 \\le T\(n/2+1\) +1 \\\\  ~
\\hspace{15 mm} \\le c\\lg\(n/2-1\)+1  \\\\  ~
\\hspace{15 mm} =clg\(n-2\) -c\\lg2 + 1 \\\\  ~
\\hspace{15 mm} \\le clg\(n-2\)
)


### Exercises 4.1-2
***
We saw that the solution of ![](http://latex.codecogs.com/gif.latex? T\(n\) = 2T\(\\lfloor n/2 \\rfloor\) + n)
is O(n lg n). Show that the solution of this recurrence is also Ω(n lg n). Conclude that the solution is Θ(n lg n).

### `Answer`
我们假设![](http://latex.codecogs.com/gif.latex? T\(n\) \\ge cn\\lg{n} )

![](http://latex.codecogs.com/gif.latex? T\(n\) = 2T\(\\lfloor n/2 \\rfloor\) + n \\\\  ~
\\hspace{15 mm} \\ge cn\(\\lg{n} - \\lg{2}\)+n \\\\  ~
\\hspace{15 mm} =cn\\lg{n} +\(1-c\\lg{2}\)n \\\\  ~
\\hspace{15 mm} \\ge cnlg\(n\)
\\\\  ~
\\hspace{15 mm} for ~ 1-c\\lg{2} < 0
)


### Exercises 4.1-3
***
Show that by making a different inductive hypothesis, we can overcome the difficulty with the boundary condition T (1) = 1 for the recurrence (4.4) without adjusting the boundary conditions for the inductive proof.

### `Answer`
我们假设 ![](http://latex.codecogs.com/gif.latex? T\(n\) \\le n\\lg{n}+n)

![](http://latex.codecogs.com/gif.latex? T\(n\) \\le 2\(c\\lfloor n/2 \\rfloor \\lg\(\\lfloor n/2 \\rfloor\) + \\lfloor n/2 \\rfloor\) + n \\\\  ~
\\hspace{15 mm} \\le 2c\(n/2\)\\lg\(n/2\) + 2\(n/2\) + n \\\\  ~
\\hspace{15 mm} \\le cn\\lg\(n/2\) + 2n \\\\  ~
\\hspace{15 mm} \\le cn\\lg{n} - \\lg{2}cn + 2n \\\\  ~
\\hspace{15 mm} \\le cn\\lg{n} + \(2-c\)n \\\\  ~
\\hspace{15 mm} \\le cn\\lg{n} + n ~~~~~~~~~~~~ for ~ c \\ge 1
)

### Exercises 4.1-4
***
Show that Θ(n lg n) is the solution to the "exact" recurrence (4.2) for merge sort.

### `Answer`
我们假设![](http://latex.codecogs.com/gif.latex? T\(n\) \\ge cn\\lg{n} )

![](http://latex.codecogs.com/gif.latex? T\(n\) \\ge 2T\(n/2\) + kn \\\\  ~
\\hspace{15 mm} =cn\\lg{n} +\(k-c\\lg{2}\)n \\\\  ~
\\hspace{15 mm} \\ge cn\\lg{n}  ~~~~~~ if ~ k \\le c\\lg{2}
)

我们假设![](http://latex.codecogs.com/gif.latex? T\(n\) \\le c\(n-2\)\\lg\(n-2\) )

![](http://latex.codecogs.com/gif.latex? T\(n\) \\le T\(n/2+1\) + T\(n/2\) + kn \\\\  ~
\\hspace{15 mm} \\le c\(n-2\)\\lg\(\\frac{n-2}{2}\) + kn \\\\  ~
\\hspace{15 mm} = c\(n-2\)\\lg\(n-2\) +kn - c\\lg{2}\(n-2\) \\\\  ~
\\hspace{15 mm} \\le c\(n-2\)\\lg\(n-2\) ~~~~~~~~if~~kn \\le c\\lg{2}\(n-2\)
) 

### Exercises 4.1-5
***
Show that the solution to ![](http://latex.codecogs.com/gif.latex? T\(n\) = 2T\(\\lfloor n/2 \\rfloor + 17\) + n ) is O(n lg n).

### `Answer`
我们假设![](http://latex.codecogs.com/gif.latex? T\(n\) \\le c\(n-a\)\\lg\(n-a\) )

![](http://latex.codecogs.com/gif.latex? T\(n\) \\le 2c\(\\lfloor n/2 \\rfloor + 17 - a\)\\lg\(\\lfloor n/2 \\rfloor + 17-a\) + n\\\\  ~
\\hspace{15 mm} \\le  2c\(n/2 +1+ 17 - a\)\\lg\( n/2 +1+ 17-a\) + n \\\\  ~
\\hspace{15 mm} \\le c\(n+36-2a\)\\lg\(\\frac{n+36-2a}{2}\)+n \\\\  ~
\\hspace{15 mm} \\le c\(n+36-2a\)\\lg\(n+36-2a\) - c\(n+36-2a\)+n \\\\  ~
\\hspace{15 mm} \\le c\(n+36-2a\)\\lg\(n+36-2a\) ~~~if ~~ c > 1 \\\\  ~ 
\\hspace{15 mm} \\le c\(n-a\)\\lg\(n-a\) ~~~~if ~~ a \ge 36
) 

### Exercises 4.1-6
***
Solve the recurrence ￼![](http://latex.codecogs.com/gif.latex? T\(n\) = 2T\(\\sqrt{n}\)+1 )
by making a change of variables. Your solution should be asymptotically tight. Do not worry about whether values are integral.

### `Answer`
设n = lgn,得到新的递归式

![](http://latex.codecogs.com/gif.latex? T\(2^n\) = 2T\(2^{n/2}\) + 1)

再令S(n) = T(2^n)可以得到

![](http://latex.codecogs.com/gif.latex? S\(n\) = S2\(m/2\) + 1)

按照前面的方法解这个递归式即可



***
Follow [@louis1992](https://github.com/gzc) on github to help finish this task.

